Fix clean target

test/Server.fst
@@ -44,6 +44,24 @@ val bufstrcmp (b: buffer char) (s: C.String.t): Stack bool
       Seq.length b >= l /\
       Seq.equal (Seq.slice b 0 (l - 1)) (Seq.slice s 0 (l - 1)))))))
 
+module S = FStar.Seq
+
+let slice_plus_one #a (s1 s2: S.seq a) (i: nat): Lemma
+  (requires (
+    i < S.length s1 /\
+    i < S.length s2 /\
+    S.equal (S.slice s1 0 i) (S.slice s2 0 i) /\
+    S.index s1 i == S.index s2 i))
+  (ensures (
+    S.equal (S.slice s1 0 (i + 1)) (S.slice s2 0 (i + 1))))
+  [ SMTPat (S.slice s1 0 (i + 1)); SMTPat (S.slice s2 0 (i + 1)) ]
+=
+  let x = S.index s1 i in
+  let s1' = S.append (S.slice s1 0 i) (S.cons x S.createEmpty) in
+  let s2' = S.append (S.slice s2 0 i) (S.cons x S.createEmpty) in
+  assert (S.equal s1' (S.slice s1 0 (i + 1)));
+  assert (S.equal s2' (S.slice s2 0 (i + 1)))
+
 let bufstrcmp b s =
   let h0 = ST.get () in
   push_frame ();
